src/PlutusIR/Semantics/Static/normaliser_STLC/alpha/util.v
@@ -92,3 +92,8 @@ Admitted.
 Lemma lookup_no_key_then_none X (sigma : list (string * term)) :
   ~ In X (map fst sigma) -> lookup X sigma = None.
 Admitted.
+
+Lemma not_existsb_not_in y U' : 
+  existsb (eqb y) (ftv U') = false -> ~ In y (ftv U').
+Proof.
+Admitted.
